src/genCoq.ml
@@ -1,0 +1,378 @@
+open Common
+open Spec
+
+let coq_of_typ = function
+  | Num -> "num"
+  | Str -> "str"
+  | Fdesc -> "fdesc"
+
+let coq_recv_typ = function
+  | Num -> "recv_num", "RecvNum"
+  | Str -> "recv_str", "RecvStr"
+  | Fdesc -> "recv_fd", "RecvFD_t"
+
+let coq_send_typ = function
+  | Num -> "send_num", "SendNum"
+  | Str -> "send_str", "SendStr"
+  | Fdesc -> "send_fd", "SendFD_t"
+
+let coq_of_string s =
+  s |> explode
+    |> List.map (mkstr "\"%c\" :: ")
+    |> String.concat ""
+    |> mkstr "(%snil)"
+
+let coq_of_expr = function
+  | Var id -> id
+  | NumLit i -> string_of_int i
+  | StrLit s -> coq_of_string s
+
+let coq_of_msg_decl m =
+  mkstr "| %s : %s" m.tag
+    (m.payload
+      |> List.map coq_of_typ
+      |> List.map (mkstr "%s -> ")
+      |> String.concat ""
+      |> mkstr "%smsg")
+
+let str_of_args m =
+  m.payload
+    |> List.mapi (fun i _ -> mkstr "p%d" i)
+    |> String.concat " "
+
+let coq_trace_recv_msg tag_map m =
+  let hdr =
+    mkstr "| %s %s =>" m.tag (str_of_args m)
+  in
+  let pay =
+    m.payload
+      |> List.mapi (fun i t ->
+          let rF, rT = coq_recv_typ t in
+          mkstr "%s c p%d ++" rT i)
+      |> List.rev
+      |> String.concat "\n"
+  in
+  let tag =
+    mkstr "RecvNum c (Num \"%03d\")"
+      (List.assoc m.tag tag_map)
+  in
+  String.concat "\n" [hdr; pay; tag]
+
+(* WARNING copy/paste of coq_trace_recv_msg *)
+let coq_trace_send_msg tag_map m =
+  let hdr =
+    mkstr "| %s %s =>" m.tag (str_of_args m)
+  in
+  let pay =
+    m.payload
+      |> List.mapi (fun i t ->
+          let sF, sT = coq_send_typ t in
+          mkstr "%s c p%d ++" sT i)
+      |> List.rev
+      |> String.concat "\n"
+  in
+  let tag =
+    mkstr "SendNum c (Num \"%03d\")"
+      (List.assoc m.tag tag_map)
+  in
+  String.concat "\n" [hdr; pay; tag]
+
+(* recv msg on bound chan "c" *)
+let coq_recv_msg tag_map m =
+  let hdr =
+    mkstr "| Num \"%03d\" => (* %s *)"
+      (List.assoc m.tag tag_map) m.tag
+  in
+  let pay =
+    let aux (i, code, tr) t =
+      let rF, rT = coq_recv_typ t in
+      ( i + 1
+      , mkstr "p%d <- %s c (tr ~~~ %s);" i rF tr :: code
+      , mkstr "%s c p%d ++ %s" rT i tr
+      )
+    in
+    let tr =
+      mkstr "RecvNum c (Num \"%03d\") ++ tr"
+        (List.assoc m.tag tag_map)
+    in
+    m.payload
+      |> List.fold_left aux (0, [], tr)
+      |> fun (_, x, _) -> x
+      |> List.rev
+      |> String.concat "\n"
+  in
+  let ret =
+    mkstr "{{ Return (%s %s) }}" m.tag (str_of_args m)
+  in
+  String.concat "\n" [hdr; pay; ret]
+
+(* send msg on bound chan "c" *)
+(* WARNING copy/paste of coq_recv_msg *)
+let coq_send_msg tag_map m =
+  let hdr =
+    String.concat "\n"
+      [ mkstr "| %s %s =>" m.tag (str_of_args m)
+      ; mkstr "send_num c (Num \"%03d\") tr;;" (List.assoc m.tag tag_map)
+      ]
+  in
+  let pay =
+    let aux (i, code, tr) t =
+      let sF, sT = coq_send_typ t in
+      ( i + 1
+      , mkstr "%s c p%d (tr ~~~ %s);;" sF i tr :: code
+      , mkstr "%s c p%d ++ %s" sT i tr
+      )
+    in
+    let tr =
+      mkstr "SendNum c (Num \"%03d\") ++ tr"
+        (List.assoc m.tag tag_map)
+    in
+    m.payload
+      |> List.fold_left aux (0, [], tr)
+      |> fun (_, x, _) -> x
+      |> List.rev
+      |> String.concat "\n"
+  in
+  let ret =
+    "{{ Return tt }}"
+  in
+  String.concat "\n" [hdr; pay; ret]
+
+let coq_of_msg_expr m =
+  mkstr "(%s %s)" m.tag
+    (m.payload
+      |> List.map coq_of_expr
+      |> String.concat ") ("
+      |> mkstr "(%s)")
+
+let coq_of_frame fr =
+  fr |> List.map (mkstr "%s * ")
+     |> String.concat ""
+     |> mkstr "%semp"
+
+let coq_of_cmd tr fr = function
+  | Send (c, m) ->
+      let fr' = remove (mkstr "bound %s" c) fr in
+      mkstr "send_msg %s %s (tr ~~~ %s) <@> %s;;"
+        c (coq_of_msg_expr m) tr (coq_of_frame fr')
+  | Call (res, f, arg) ->
+      mkstr "%s <- call %s %s (tr ~~~ %s) <@> %s;"
+        res (coq_of_string f) (coq_of_expr arg) tr (coq_of_frame fr)
+
+let coq_trace_of_cmd = function
+  | Send (c, m) ->
+      mkstr "SendMsg %s %s ++ "
+        c (coq_of_msg_expr m)
+  | Call (res, f, arg) ->
+      mkstr "Call_t %s %s %s ++ "
+        (coq_of_string f) (coq_of_expr arg) res
+
+let coq_of_prog tr fr p =
+  let rec loop code tr = function
+    | Nop ->
+        (String.concat "\n" (List.rev code), tr)
+    | Seq (c, p') ->
+        let cd' = coq_of_cmd tr fr c :: code in
+        let tr' = coq_trace_of_cmd c ^ tr in
+        loop cd' tr' p'
+  in
+  loop [] tr p
+
+let rec coq_trace_of_prog = function
+  | Nop -> []
+  | Seq (c, p') -> coq_trace_of_cmd c :: coq_trace_of_prog p'
+
+let expr_vars = function
+  | Var id -> [id]
+  | _ -> []
+
+let cmd_vars = function
+  | Send (c, m) ->
+      c :: List.flatten (List.map expr_vars m.payload)
+  | Call (var, func, arg) ->
+      var :: expr_vars arg
+
+let rec prog_vars = function
+  | Nop -> []
+  | Seq (c, p) -> cmd_vars c @ prog_vars p
+
+let coq_of_msg_pat m =
+  mkstr "| %s %s =>" m.tag
+    (String.concat " " m.payload)
+
+let handler_vars h =
+  let c, m = h.trigger in
+  uniq (c :: m.payload @ prog_vars h.respond)
+
+let coq_spec_of_handler h =
+  let c, m = h.trigger in
+  let hdr =
+    mkstr "| VE_%s :\nforall %s,\nValidExchange ("
+      m.tag (String.concat " " (handler_vars h))
+  in
+  let bdy =
+    h.respond
+      |> coq_trace_of_prog
+      |> List.rev
+      |> String.concat "\n"
+      |> function "" -> "(* no response *)" | x -> x
+  in
+  let ftr =
+    mkstr "RecvMsg %s (%s %s))"
+      c m.tag (String.concat " " m.payload)
+  in
+  String.concat "\n" [hdr; bdy; ftr]
+
+let coq_of_handler h =
+  let c, m = h.trigger in
+  let tr =
+    mkstr "RecvMsg %s (%s %s) ++ tr"
+      c m.tag (String.concat " " m.payload)
+  in
+  let fr =
+    [ mkstr "bound %s" c ]
+  in
+  let code, tr =
+    coq_of_prog tr fr h.respond
+  in
+  String.concat "\n"
+    [ coq_of_msg_pat m
+    ; code
+    ; mkstr "{{ Return (tr ~~~ %s) }}" tr
+    ]
+
+(* coq template has string holes for
+ *  1. declaring msg
+ *  2. RecvMsg cases
+ *  3. SendMsg cases
+ *  4. recv_msg cases
+ *  5. send_msg cases
+ *  6. ValidExchange cases
+ *  7. exchange cases
+ *)
+let coq_template = format_of_string "
+Require Import List.
+Require Import Ascii.
+Require Import Ynot.
+Require Import KrakenBase.
+
+Open Local Scope char_scope.
+Open Local Scope hprop_scope.
+Open Local Scope stsepi_scope.
+
+Inductive msg : Set :=
+%s
+(* special case for errors *)
+| BadTag : num -> msg.
+
+Definition RecvMsg (c : chan) (m : msg) : Trace :=
+  match m with
+%s
+    (* special case for errors *)
+    | BadTag p0 =>
+      RecvNum c p0
+  end.
+
+(* prevent sep tactic from unfolding *)
+Global Opaque RecvMsg.
+
+Definition SendMsg (c : chan) (m : msg) : Trace :=
+  match m with
+%s
+    (* special case for errors *)
+    | BadTag p0 =>
+      SendNum c (Num \"000\")
+  end.
+
+(* prevent sep tactic from unfolding *)
+Global Opaque SendMsg.
+
+Definition recv_msg :
+  forall (c : chan) (tr : [Trace]),
+  STsep (tr ~~ traced tr * bound c)
+        (fun (m : msg) => tr ~~ traced (RecvMsg c m ++ tr) * bound c).
+Proof.
+  intros; refine (
+    tag <- recv_num c tr;
+    match tag with
+%s
+      (* special case for errors *)
+      | m =>
+        {{ Return (BadTag m) }}
+    end
+  );
+  sep fail auto;
+  repeat rewrite app_ass; simpl;
+  sep fail auto.
+Qed.
+
+Definition send_msg :
+  forall (c : chan) (m : msg) (tr : [Trace]),
+  STsep (tr ~~ traced tr * bound c)
+        (fun (_ : unit) => tr ~~ traced (SendMsg c m ++ tr) * bound c).
+Proof.
+  intros; refine (
+    match m with
+%s
+      (* special case for errors *)
+      | BadTag _ =>
+        send_num c (Num \"000\") tr;;
+        {{ Return tt }}
+    end
+  );
+  sep fail auto;
+  repeat rewrite app_ass; simpl;
+  sep fail auto.
+Qed.
+
+Inductive ValidExchange : Trace -> Prop :=
+%s
+(* special case for errors *)
+| VE_BadTag :
+  forall c tag,
+  ValidExchange (
+    RecvMsg c (BadTag tag)).
+
+Inductive AddedValidExchange : Trace -> Trace -> Prop :=
+| AVE_intro :
+  forall tr1 tr2,
+  ValidExchange tr2 ->
+  AddedValidExchange tr1 (tr2 ++ tr1).
+
+Definition exchange :
+  forall (c : chan) (tr : [Trace]),
+  STsep (tr ~~ traced tr * bound c)
+        (fun (tr' : [Trace]) => tr' ~~ tr ~~ traced tr' * [AddedValidExchange tr tr'] * bound c).
+Proof.
+  intros; refine (
+    req <- recv_msg c tr;
+    match req with
+%s
+      (* special case for errors *)
+      | BadTag tag =>
+        {{ Return (tr ~~~ RecvMsg c (BadTag tag) ++ tr) }}
+    end
+
+  );
+  sep fail auto;
+    apply himp_pure';
+    repeat rewrite -> app_assoc;
+    constructor; auto;
+    repeat rewrite <- app_assoc;
+    constructor; auto.
+Qed.
+"
+
+let coq_of_spec s =
+  let m = gen_tag_map s in
+  let fmt l f =
+    String.concat "\n" (List.map f l)
+  in
+  mkstr coq_template
+    (fmt s.msg_decl coq_of_msg_decl)
+    (fmt s.msg_decl (coq_trace_recv_msg m))
+    (fmt s.msg_decl (coq_trace_send_msg m))
+    (fmt s.msg_decl (coq_recv_msg m))
+    (fmt s.msg_decl (coq_send_msg m))
+    (fmt s.protocol coq_spec_of_handler)
+    (fmt s.protocol coq_of_handler)
